cp

examples/generic/Interop.fst
@@ -1,4 +1,5 @@
 module Interop
+open FStar.FunctionalExtensionality
 open FStar.Integers
 module L = LowStar.Buffer
 module M = FStar.Map
@@ -28,7 +29,7 @@ let as_reg (n:ireg) =
 let rec arrow (args: list Type) (result:Type) =
   match args with
   | [] -> result
-  | a :: rest -> (a -> arrow rest result)
+  | a :: rest -> (a ^-> arrow rest result)
 
 let vale_args = n:list (a:Type0{a == uint_64}){List.Tot.length n <= 4}
 
@@ -39,28 +40,17 @@ let rec n_arrow (n:arity) (result:Type) =
   if n = 0 then result
   else uint_64 -> n_arrow (n - 1) result
 
-
 let elim #n #result (f:n_arrow n result)
   : normalize_term (n_arrow n result)
   = f
-
+  
+module F = FStar.FunctionalExtensionality
 let elim_1 (#n:arity{n > 0}) #r (f:n_arrow n r)
-  : uint_64 -> n_arrow (n - 1) r
+  : (uint_64 -> n_arrow (n - 1) r)
   = f
 
-let rec widen_2 (#n:arity) (#r:Type) (f:n_arrow n r) (m:arity{n <= m})
-  : Tot (n_arrow m r) (decreases m) =
-  if m = n then f
-  else (fun (x:uint_64) -> widen_2 f (m - 1))
-
-let rec widen (#n:arity) (#r:Type) (f:n_arrow n r) (m:arity{n <= m})
-  : Tot (n_arrow m r) (decreases m) =
-  if m = n then f
-  else if n = 0 then (fun (x:uint_64) -> widen f (m - 1))
-  else fun (x:uint_64) -> widen #(n - 1) #r (elim_1 f x) (m - 1)
-
 let rec elim_m (#n:arity) #r (m:arity{m <= n}) (f:n_arrow n r)
-  : registers -> n_arrow m r
+  : (registers -> n_arrow m r)
   = fun regs ->
       match (n - m) with
       | 0 -> f
@@ -106,80 +96,35 @@ let rec as_lowstar_sig (n:arity{n > 0}) (pre:vale_pre n) (post:vale_post n) : Ty
 assume val gput: f:(unit -> GTot HS.mem) -> ST unit (requires (fun _ -> True)) (ensures (fun _ _ h1 -> h1 == f()))
 assume val put: h:HS.mem -> ST unit (requires (fun _ -> True)) (ensures (fun _ _ h1 -> h1 == h))
 
-module List = FStar.List.Tot
-
-// let rec elim_l (#n:arity{n > 0}) #r (m:arity{0 < m /\ m <= n}) (f:n_arrow n r)
-//   : List.llist uint_64 (n - m) -> n_arrow m r
-//   = fun nl ->
-//       match (n - m) with
-//       | 0 -> f
-//       | _ -> elim_l #(n - 1) #r m (elim_1 f (List.hd nl)) (List.tl nl)
-
-
-// let rec list_as_registers (m:arity) (l:List.llist uint_64 m) : registers =
-//   match l with
-//   | [] -> Map.const 0uL
-//   | hd::tl ->
-//     let tl = list_as_registers (m - 1) tl in
-//     let reg = as_reg (1 + max_arity - m) in
-//     Map.upd tl reg hd
-
+// module List = FStar.List.Tot
+#reset-options "--z3rlimit_factor 10 --max_fuel 6 --initial_fuel 6 --max_ifuel 6 --initial_ifuel 6"
 
 let idem_elim_m (#n:arity) (m1:arity{m1 <= n}) (m2:arity{m2 <= m1}) (f:vale_pre n) regs h
    : Lemma (elim_m 0 (elim_m m2 (elim_m m1 f regs) regs) regs h <==> (elim_m 0 (elim_m m2 f regs) regs h))
    = ()
 
-let widen_elim_m (#n:arity) (m1:arity{m1 <= n}) (m2:arity{m2 <= m1}) (f:vale_pre n) regs h
-   : Lemma (elim_m 0 (widen (elim_m 0 f regs) max_arity) regs h <==> elim_m 0 f regs h)
-   = ()
+// let widen_elim_m (#n:arity) (m1:arity{m1 <= n}) (m2:arity{m2 <= m1}) (f:vale_pre n) regs h
+//    : Lemma (elim_m 0 (widen (elim_m 0 f regs) max_arity) regs h <==> elim_m 0 f regs h)
+//    = ()
 
-module F = FStar.FunctionalExtensionality
+let rec elim_1_m_aux (#n:arity{n > 0}) (m:arity{m = 1 /\ m <= n}) (pre0:vale_pre n) (regs:registers) (x:uint_64) h
+  : Lemma (ensures (let regs1 = Map.upd regs (as_reg 1) x in
+                    elim_m 0 pre0 regs1 h <==>
+                    elim_m 0 (elim_m m pre0 regs1) regs1 h))
+  = ()                    
 
-// let elim_m_elim (#n:arity{n > 0}) (#pre:vale_pre n) (#post:vale_post n)
-//                 (v:vale_sig n pre post)
-//     : Lemma (elim_m n pre (Map.const 0uL) == elim (elim_m n
-//             (ensures (elim
+let rec elim_1_m (#n:arity{n > 0}) (m:arity{m = 1 /\ m <= n}) (pre0:vale_pre n) (regs:registers) (x:uint_64) h
+  : Lemma (ensures (let regs1 = Map.upd regs (as_reg 1) x in
+                    elim_m 0 pre0 regs1 h <==>
+                    elim_m 0 (elim_m m pre0 regs) regs1 h))
+  = admit()                    
 
-// let elim_m_pre (#n:arity) (#r:Type)
-//                (f:n_arrow n r)
-//                (m:arity{0 < m /\ m <= n})
-//                (regs:registers)
-//   : Lemma (elim_m
-// val elim_m_pre (#n:arity) (m:arity{0 < m /\ m <= n /\ m = 1}) (pre:vale_pre n) (regs:registers) (x:uint_64) (h:HS.mem)
-//   : Lemma (requires (elim #1 (elim_m m pre regs) x h))
-//           (ensures  (elim_m 0 pre (Map.upd regs R1 x) h))
-//   = admit()
-//   = match n - m with
-//     | 0 ->
-//       assert (elim_m m pre regs
-//     | _ -> admit()
-#reset-options "--z3rlimit_factor 10 --max_fuel 6 --initial_fuel 6 --max_ifuel 6 --initial_ifuel 6"
-
-// let rec elim_m_elim_vale_pre
-//                  (n:arity)
-//                  (pre0:vale_pre n)
-//                  (h:HS.mem)
-//                  (regs:registers{elim_m 0 pre0 regs h})
-//     : Lemma (as_vale_pre (widen_2 pre0 4) ({registers=regs; memory=h}))
-//     = match m - n with
-//       | 0 -> ()
-//       | _ -> let pre1 = elim_1 pre0 (Map.sel regs (as_reg (1 + max_arity - n))) in
-//             assert (elim_m 0 pre1 regs h);
-//             elim_m_elim_vale_pre (n - 1) pre1 h regs;
-//             assert (as_vale_pre (widen2 pre1 4) ({registers=regs; memory=h}))
-
-// let elim_m_widen_post (n:arity{0 < n})
-//                       (m:arity{m = 1})
-//                       (post0:vale_post n)
-//                       (regs:registers)
-//                       (h:HS.mem)
-//                       (state1:state)
-//     : Lemma (let post : n_arrow 1 (HS.mem -> HS.mem -> prop) = elim_m m post0 regs in
-//              let state = { registers = regs; memory = h } in
-//              as_vale_post (widen post 4) state state1 <==>
-//              as_vale_post (widen post0 4) state state1)
-//     = admit()
-
+let rec elim_1_m_ (#n:arity{n > 0}) (m:arity{m = 1 /\ m <= n}) (pre0:vale_pre n) (regs:registers) (x:uint_64) h
+  : Lemma (ensures (let regs1 = Map.upd regs (as_reg 4) x in
+                    elim_m 0 pre0 regs1 h <==>
+                    elim #1 (elim_m m pre0 regs) x h))
+  = ()
+           
 let rec wrap
         (#n:arity{n > 0})
         (#pre:vale_pre n)
@@ -187,13 +132,7 @@ let rec wrap
         (v:vale_sig n pre post)
   : as_lowstar_sig n pre post
   =
-  let rec aux (m:arity{0 < m /\ m <= n}) (regs:registers{
-          let pre0 = pre in
-          let pre : vale_pre m = elim_m m pre0 regs in
-          (forall h.
-             elim_m 0 pre0 regs h <==>
-             elim_m 0 pre regs h)
-      })
+  let rec aux (m:arity{0 < m /\ m <= n}) (regs:registers)
     : Tot (as_lowstar_sig m (elim_m m pre regs) (elim_m m post regs))
     = let pre0 = pre in
       let post0 = post in
@@ -208,35 +147,32 @@ let rec wrap
             fun (x:uint_64) ->
               let h0 = get () in
               let state = {
-                registers = Map.upd regs (as_reg m) x;
+                registers = Map.upd regs (as_reg (1 + max_arity - m)) x;
                 memory = h0;
               } in
-              assert (elim #1 pre x h0);
-              // elim_m_elim_vale_pre n 1 pre0 x h0 regs;
-              // assert (as_vale_pre (widen pre 4) state);
-              // elim_m_widen_pre n m pre0 state.registers h0;
-              assert (as_vale_pre (widen pre0 4) state);
+              // assert (elim #1 pre x h0);
+              // elim_1_m m pre0 regs x h0;
+              // assert (elim_m 0 pre0 state.registers h0);
               let state1 = v state in
-              assert (as_vale_post (widen post0 4) state (v state));
-              admit();
-              // elim_m_widen_post n m post0 state.registers h0 (v state);
-              assert (as_vale_post (widen post 4) state (v state));
+              // assert (as_vale_post post0 state (v state));
+              //assume (as_vale_post post state (v state));
+              //assume (elim #1 post x h0 (v state).memory);
               put (v state).memory
        in
        (f <: as_lowstar_sig 1 pre post)
 
     | _ ->
-      admit()
-    in
-    admit()
-
       let f : x:uint_64
               -> as_lowstar_sig
                    (m - 1)
-                   (elim_m (m - 1) (elim_1 pre x) regs)
-                   (elim_m (m - 1) (elim_1 post x) regs) =
+                   (elim_1 pre x)
+                   (elim_1 post x) =
           fun (x:uint_64) ->
-            aux (m - 1) (Map.upd regs (as_reg m) x)
+            let regs1 = (Map.upd regs (as_reg (1 + max_arity - m)) x) in
+            let f : as_lowstar_sig (m - 1) (elim_m (m - 1) pre0 regs1) (elim_m (m - 1) post0 regs1) = aux (m - 1) regs1 in
+            // assume (elim_m (m - 1) pre0 regs1 == elim_1 pre x);
+            // assume (elim_m (m - 1) post0 regs1 == elim_1 post x);
+            f
       in
       f
     in
